A bit of work on emulate.

BackTrans/Emulate.v
@@ -24,16 +24,59 @@ Fixpoint emulate (n : nat) (t : U.UTm) : S.Tm :=
     | U.wrong => stlcOmega (UVal n)
     | U.var i => S.var i
     | U.abs t => inArrDwn n (S.abs (UVal n) (emulate n t))
-    | U.app t₁ t₂ => S.unit
+    | U.app t₁ t₂ => S.app (caseArrUp n (emulate n t₁)) (emulate n t₂)
     | U.unit => inUnitDwn n S.unit
     | U.true => inBoolDwn n S.true
     | U.false => inBoolDwn n S.false
-    | U.ite t₁ t₂ t₃ => S.unit
+    | U.ite t₁ t₂ t₃ => S.ite (caseBoolUp n (emulate n t₁)) (emulate n t₂) (emulate n t₃)
     | U.pair t₁ t₂ => inProdDwn n (S.pair (emulate n t₁) (emulate n t₂))
-    | U.proj₁ t => S.unit
-    | U.proj₂ t => S.unit
-    | U.inl t => inSumDwn n (emulate n t)
-    | U.inr t => inSumDwn n (emulate n t)
-    | U.caseof t₁ t₂ t₃ => S.unit
-    | U.seq t₁ t₂ => S.unit
+    | U.proj₁ t => S.proj₁ (caseProdUp n (emulate n t))
+    | U.proj₂ t => S.proj₂ (caseProdUp n (emulate n t))
+    | U.inl t => inSumDwn n (S.inl (emulate n t))
+    | U.inr t => inSumDwn n (S.inr (emulate n t))
+    | U.caseof t₁ t₂ t₃ => S.caseof (caseSumUp n (emulate n t₁)) (emulate n t₂) (emulate n t₃)
+    | U.seq t₁ t₂ => S.seq (caseUnitUp n (emulate n t₁)) (emulate n t₂)
   end.
+
+Fixpoint emulate_pctx (n : nat) (t : U.PCtx) : S.PCtx :=
+  match t with
+    | U.phole => S.phole
+    | U.pabs C => S.phole (* inArrDwn n (S.pabs (UVal n) (emulate_pctx n C)) *)
+    | U.papp₁ C t₂ => S.papp₁ S.phole (* (caseArrUp n (emulate_pctx n C)) *) (emulate n t₂)
+    | U.papp₂ t₁ C => S.papp₂ (caseArrUp n (emulate n t₁)) (emulate_pctx n C)
+    | U.pite₁ C₁ t₂ t₃ => S.pite₁ S.phole (* (caseBoolUp n (emulate_pctx n C₁)) *) (emulate n t₂) (emulate n t₃)
+    | U.pite₂ t₁ C₂ t₃ => S.pite₂ (caseBoolUp n (emulate n t₁)) (emulate_pctx n C₂) (emulate n t₃)
+    | U.pite₃ t₁ t₂ C₃ => S.pite₃ (caseBoolUp n (emulate n t₁)) (emulate n t₂) (emulate_pctx n C₃)
+    | U.ppair₁ C₁ t₂ => S.phole (* inProdDwn n (S.ppair₁ (emulate_pctx n C₁) (emulate n t₂)) *)
+    | U.ppair₂ t₁ C₂ => S.phole (* inProdDwn n (S.ppair₂ (emulate n t₁) (emulate_pctx n C₂)) *)
+    | U.pproj₁ C => S.phole (* S.pproj₁ (caseProdUp n (emulate_pctx n C)) *)
+    | U.pproj₂ C => S.phole (* S.pproj₂ (caseProdUp n (emulate_pctx n C)) *)
+    | U.pinl C => S.phole (* inSumDwn n (S.pinl (emulate_pctx n C)) *)
+    | U.pinr C => S.phole (* inSumDwn n (S.pinr (emulate_pctx n C)) *)
+    | U.pcaseof₁ C₁ t₂ t₃ => S.phole (* S.pcaseof₁ (caseSumUp n (emulate_pctx n C₁)) (emulate n t₂) (emulate n t₃) *)
+    | U.pcaseof₂ t₁ C₂ t₃ => S.pcaseof₂ (caseSumUp n (emulate n t₁)) (emulate_pctx n C₂) (emulate n t₃)
+    | U.pcaseof₃ t₁ t₂ C₃ => S.pcaseof₃ (caseSumUp n (emulate n t₁)) (emulate n t₂) (emulate_pctx n C₃)
+    | U.pseq₁ C₁ t₂ => S.phole (* S.seq (caseUnitUp n (emulate_pctx n C₁)) (emulate n t₂) *)
+    | U.pseq₂ t₁ C₂ => S.pseq₂ (caseUnitUp n (emulate n t₁)) (emulate_pctx n C₂)
+  end.
+
+Fixpoint toUVals n (Γ : Dom) : Env :=
+  match Γ with
+      0 => S.empty
+    | S Γ' => toUVals n Γ' ▻ UVal n
+  end.
+
+Lemma toUVals_entry {n Γ i} :
+  Γ ∋ i → ⟪ i : UVal n ∈ toUVals n Γ ⟫.
+Proof.
+  induction 1; simpl; crushTyping.
+Qed.
+
+Lemma emulate_T {n Γ t} :
+  ⟨ Γ ⊢ t ⟩ →
+  ⟪ toUVals n Γ ⊢ emulate n t : UVal n ⟫.
+Proof.
+  induction 1;
+  eauto using stlcOmegaT, toUVals_entry with typing uval_typing.
+Qed.
+
