BackTrans/UValHelpers.v
@@ -29,6 +29,44 @@ Section Intro.
   Definition inSumDwn (n : nat) (t : Tm) := app (downgrade n 1) (inSum n t).
 End Intro.
 
+Section IntroTypes.
+  Lemma inUnitDwn_T {n t Γ} : ⟪ Γ ⊢ t : tunit ⟫ → ⟪ Γ ⊢ inUnitDwn n t : UVal n ⟫.
+  Proof.
+    unfold inUnitDwn.
+    eauto using upgrade_T1, downgrade_T1 with typing uval_typing.
+  Qed.
+
+  Lemma inBoolDwn_T {n t Γ} : ⟪ Γ ⊢ t : tbool ⟫ → ⟪ Γ ⊢ inBoolDwn n t : UVal n ⟫.
+  Proof.
+    unfold inBoolDwn.
+    eauto using upgrade_T1, downgrade_T1 with typing uval_typing.
+  Qed.
+
+  Lemma inProdDwn_T {n t Γ} : ⟪ Γ ⊢ t : UVal n × UVal n ⟫ → ⟪ Γ ⊢ inProdDwn n t : UVal n ⟫.
+  Proof.
+    unfold inProdDwn.
+    eauto using upgrade_T1, downgrade_T1 with typing uval_typing.
+  Qed.
+
+  Lemma inSumDwn_T {n t Γ} : ⟪ Γ ⊢ t : UVal n ⊎ UVal n ⟫ → ⟪ Γ ⊢ inSumDwn n t : UVal n ⟫.
+  Proof.
+    unfold inSumDwn.
+    eauto using upgrade_T1, downgrade_T1 with typing uval_typing.
+  Qed.
+
+  Lemma inArrDwn_T {n t Γ} : ⟪ Γ ⊢ t : UVal n ⇒ UVal n ⟫ → ⟪ Γ ⊢ inArrDwn n t : UVal n ⟫.
+  Proof.
+    unfold inArrDwn.
+    eauto using upgrade_T1, downgrade_T1 with typing uval_typing.
+  Qed.
+End IntroTypes.
+
+Hint Resolve inUnitDwn_T : uval_typing.
+Hint Resolve inBoolDwn_T : uval_typing.
+Hint Resolve inProdDwn_T : uval_typing.
+Hint Resolve inSumDwn_T : uval_typing.
+Hint Resolve inArrDwn_T : uval_typing.
+
 Section IntroProps.
   Lemma termrel_inUnitDwn {d w n p vs vu} :
     dir_world_prec n w d p →
@@ -92,12 +130,51 @@ Section IntroProps.
 End IntroProps.
 
 Section Destruct.
-  Definition caseUnitDwn (n : nat) (t : Tm) := caseUnit n (app (downgrade n 1) t).
-  Definition caseBoolDwn (n : nat) (t : Tm) := caseBool n (app (downgrade n 1) t).
-  Definition caseProdDwn (n : nat) (t : Tm) := caseProd n (app (downgrade n 1) t).
-  Definition caseSumDwn (n : nat) (t : Tm) := caseSum n (app (downgrade n 1) t).
-  Definition caseArrDwn (n : nat) (t : Tm) := caseArr n (app (downgrade n 1) t).
+  Definition caseUnitUp (n : nat) (t : Tm) := caseUnit n (app (upgrade n 1) t).
+  Definition caseBoolUp (n : nat) (t : Tm) := caseBool n (app (upgrade n 1) t).
+  Definition caseProdUp (n : nat) (t : Tm) := caseProd n (app (upgrade n 1) t).
+  Definition caseSumUp (n : nat) (t : Tm) := caseSum n (app (upgrade n 1) t).
+  Definition caseArrUp (n : nat) (t : Tm) := caseArr n (app (upgrade n 1) t).
 End Destruct.
+
+Section DestructTypes.
+  Lemma caseUnitUp_T {n t Γ} : ⟪ Γ ⊢ t : UVal n ⟫ → ⟪ Γ ⊢ caseUnitUp n t : tunit ⟫.
+  Proof.
+    unfold caseUnitUp.
+    eauto using upgrade_T1, downgrade_T1 with typing uval_typing.
+  Qed.
+
+  Lemma caseBoolUp_T {n t Γ} : ⟪ Γ ⊢ t : UVal n ⟫ → ⟪ Γ ⊢ caseBoolUp n t : tbool ⟫.
+  Proof.
+    unfold caseBoolUp.
+    eauto using upgrade_T1, downgrade_T1 with typing uval_typing.
+  Qed.
+
+  Lemma caseProdUp_T {n t Γ} : ⟪ Γ ⊢ t : UVal n ⟫ → ⟪ Γ ⊢ caseProdUp n t : UVal n × UVal n ⟫.
+  Proof.
+    unfold caseProdUp.
+    eauto using upgrade_T1, downgrade_T1 with typing uval_typing.
+  Qed.
+
+  Lemma caseSumUp_T {n t Γ} : ⟪ Γ ⊢ t : UVal n ⟫ → ⟪ Γ ⊢ caseSumUp n t : UVal n ⊎ UVal n ⟫.
+  Proof.
+    unfold caseSumUp.
+    eauto using upgrade_T1, downgrade_T1 with typing uval_typing.
+  Qed.
+
+  Lemma caseArrUp_T {n t Γ} : ⟪ Γ ⊢ t : UVal n ⟫ → ⟪ Γ ⊢ caseArrUp n t : UVal n ⇒ UVal n ⟫.
+  Proof.
+    unfold caseArrUp.
+    eauto using upgrade_T1, downgrade_T1 with typing uval_typing.
+  Qed.
+
+End DestructTypes.
+
+Hint Resolve caseUnitUp_T : uval_typing.
+Hint Resolve caseBoolUp_T : uval_typing.
+Hint Resolve caseProdUp_T : uval_typing.
+Hint Resolve caseSumUp_T : uval_typing.
+Hint Resolve caseArrUp_T : uval_typing.
 
 Local Ltac crush :=
   repeat (
@@ -177,5 +254,73 @@ Section DestructProps.
       right.
       eauto using evalToStar, U.eval₀_to_eval with eval.
   Qed.
+
+  Lemma invert_valrel_pEmulDV_for_caseUValBool {d w n p vs vu} :
+    valrel d w (pEmulDV (S n) p) vs vu →
+    (∃ vs', vs = (inBool n vs') ∧ 
+                caseBool n vs -->* vs' ∧
+                valrel d w ptbool vs' vu) ∨
+    (p = imprecise ∧ (caseBool n vs) ⇑) ∨
+    (vu ≠ U.true ∧ vu ≠ U.false ∧ (caseBool n vs) ⇑).
+  Proof.
+    intros vr.
+    apply invert_valrel_pEmulDV in vr.
+    destruct vr as [[? ?] | (vs' & cases)]; 
+      subst; unfold caseBool.
+    - right. left.
+      eauto using divergence_closed_under_evalstar, caseUVal_eval_unk, stlcOmega_div.
+    - assert (cases' : (vs = inBool n vs' ∧ valrel d w ptbool vs' vu)
+                       ∨ (vs = inUnit n vs' ∧ valrel d w ptunit vs' vu)
+                       ∨ (vs = inProd n vs' ∧ valrel d w (ptprod (pEmulDV n p) (pEmulDV n p)) vs' vu)
+                       ∨ (vs = inSum n vs' ∧ valrel d w (ptsum (pEmulDV n p) (pEmulDV n p)) vs' vu)
+                       ∨ vs = inArr n vs' ∧ valrel d w (ptarr (pEmulDV n p) (pEmulDV n p)) vs' vu)
+        by (destruct cases as [?|[?|?]]; auto).
+      destruct cases' as [[? vr] | other_cases].
+      + left. destruct (valrel_ptbool_inversion vr); subst;
+        exists vs';
+        change vs' with ((var 0) [beta1 vs']) at 4;
+        assert (S.Value vs') by (destruct H0; subst; crush);
+        eauto using caseUVal_eval_bool. 
+      + right. right.
+        enough (vu ≠ U.true ∧ vu ≠ U.false ∧ caseBool n vs -->* stlcOmega tbool) as (? & ? & ?)
+            by eauto using divergence_closed_under_evalstar, stlcOmega_div.
+        destruct other_cases as [ [? vr] | [ [? vr] | [[? vr] | [? vr]]]];
+          destruct (valrel_implies_Value vr); subst;
+          crush;
+          repeat match goal with
+                     [ |- context [ ((stlcOmega ?tau) [?γ]) ] ]=> rewrite stlcOmega_sub
+                   | [ H : _ ∧ _ |- _ ]=> destruct H
+                   | [ H : ∃ _, _ |- _ ]=> destruct H
+                   | [ H : _ ∨ _ |- _ ]=> destruct H
+                   | [ |- caseBool _ (_ _ ?vs') -->* stlcOmega tbool   ] => 
+                     (replace (stlcOmega tbool) with ((stlcOmega tbool )[ beta1 vs' ]) by eapply stlcOmega_sub;
+                      eauto using caseUVal_eval_unit, caseUVal_eval_bool, caseUVal_eval_prod, caseUVal_eval_sum, caseUVal_eval_arr)
+                 end;
+          subst; try inversion 1.
+  Qed.
+
+  (* Lemma termrel_caseUValBool {d w n p vs vu}: *)
+  (*   dir_world_prec n w d p → *)
+  (*   valrel d w (pEmulDV (S n) p) vs vu → *)
+  (*   termrel d w ptbool (caseBool n vs) (U.ite vu U.true U.false). *)
+  (* Proof. *)
+  (*   unfold caseBool. *)
+  (*   intros dwp vr. *)
+  (*   destruct (valrel_implies_Value vr). *)
+  (*   apply invert_valrel_pEmulDV_for_caseUValBool in vr. *)
+  (*   destruct vr as [(? & ? & ?)|[(? & ?)|(? & ?)]]. *)
+  (*   - subst. *)
+  (*     eapply termrel_antired_star. *)
+  (*     + eapply caseUVal_eval_bool; crush. *)
+  (*     + eapply evalToStar. *)
+  (*       eapply U.eval₀_ctxeval. *)
+  (*       eauto with eval. *)
+  (*     + simpl; crush. *)
+  (*   - subst; eapply dwp_imprecise in dwp; subst. *)
+  (*     eapply (termrel_div_lt H2). *)
+  (*   - apply (termrel_div_wrong H2). *)
+  (*     right. *)
+  (*     eauto using evalToStar, U.eval₀_to_eval with eval. *)
+  (* Qed. *)
 
 End DestructProps.
